Before generalizing the regex in matchPartial_inBounds_le

Regex/Algorithm/Defs.lean
@@ -1,95 +1,100 @@
 import Regex.Parse
 
 namespace Regex
-variable {α : Type u} [deq : DecidableEq α] {r : Regex α} {w : List α}
+variable {α : Type u} [deq : DecidableEq α] {r : Regex α}
 
 /-- Various actions the match stack can execute -/
-inductive Action {α : Type u} (w : List α) : Type u where
+inductive Action (α : Type u) : Type u where
   /-- Start a regex match (and maybe finish it). -/
-  | regex (r : Regex α) (s : Pos w) (cap : Captures w) : Action w
+  | regex (r : Regex α) (w : List α) (s : ℕ) (cap : Captures) : Action α
   /-- Wait for matches from the first regex of a concatenation -/
-  | concatWait (q : Regex α) (r : Regex α) (s : Pos w) : Action w
+  | concatWait (q : Regex α) (r : Regex α) (w : List α) (s : ℕ) : Action α
   /-- Process the second regex with another match -/
-  | concat (r : Regex α) (s : Pos w) (old new : PartialMatches w) : Action w
+  | concat (r : Regex α) (w : List α) (s : ℕ) (old new : PartialMatches) : Action α
   /-- Wait for matches from the first regex of an alternation -/
-  | orWait (r : Regex α) (s : Pos w) (cap : Captures w) : Action w
+  | orWait (r : Regex α) (w : List α) (s : ℕ) (cap : Captures) : Action α
   /-- Concatenate the two lists of matches -/
-  | or (s : Pos w) (fst : PartialMatches w) : Action w
+  | or (s : ℕ) (fst : PartialMatches) : Action α
   /-- Filter matches for emptiness -/
-  | filterEmpty (emp : Bool) (s : Pos w) : Action w
+  | filterEmpty (emp : Bool) (s : ℕ) : Action α
   /-- Capture a match -/
-  | capture (n : ℕ) (s : Pos w) : Action w
+  | capture (n : ℕ) (s : ℕ) : Action α
   deriving Repr
 
 /-- A stack of actions, along with an argument -/
 @[ext]
-structure MatchStack (w : List α) where
-  entries : List (Action w)
-  arg : PartialMatches w
+structure MatchStack (α : Type*) where
+  entries : List (Action α)
+  arg : PartialMatches
   deriving Repr
 
-def Action.process (ac : Action w) (arg : PartialMatches w)
-    : MatchStack w := match ac with
-  | Action.regex r s cap => match r with
+def Action.process (ac : Action α) (arg : PartialMatches)
+    : MatchStack α := match ac with
+  | Action.regex r w s cap => match r with
     | .bot => ⟨[], []⟩
     | .empty => ⟨[], [(s, cap)]⟩
-    | .unit c => ⟨[], if h : w[s.val]? = c then [(s.succOfIndex h, cap)] else []⟩
-    | .concat q r => ⟨[regex q s cap, concatWait q r s], []⟩
-    | .or q r => ⟨[regex q s cap, orWait r s cap], []⟩
-    | .filterEmpty emp r => ⟨[regex r s cap, filterEmpty emp s], []⟩
+    | .unit c => ⟨[], if h : w[s]? = c then [(s + 1, cap)] else []⟩
+    | .concat q r => ⟨[regex q w s cap, concatWait q r w s], []⟩
+    | .or q r => ⟨[regex q w s cap, orWait r w s cap], []⟩
+    | .filterEmpty emp r => ⟨[regex r w s cap, filterEmpty emp s], []⟩
     | .star t r => match t with
-      | .greedy => ⟨[regex [/(⟨r⟩ •ε | (⟨r⟩ -ε)⟨r⟩*‹t›) | ε/] s cap], []⟩
-      | .lazy => ⟨[regex [/ε | (⟨r⟩ •ε | (⟨r⟩ -ε)⟨r⟩*‹t›)/] s cap], []⟩
+      | .greedy => ⟨[regex [/(⟨r⟩ •ε | (⟨r⟩ -ε)⟨r⟩*‹t›) | ε/] w s cap], []⟩
+      | .lazy => ⟨[regex [/ε | (⟨r⟩ •ε | (⟨r⟩ -ε)⟨r⟩*‹t›)/] w s cap], []⟩
     | .start => ⟨[], if s = 0 then [(s, cap)] else []⟩
-    | .end' => ⟨[], if s = s.end' then [(s, cap)] else []⟩
-    | .capture n r => ⟨[regex r s cap, capture n s], []⟩
+    | .end' => ⟨[], if s = w.length then [(s, cap)] else []⟩
+    | .capture n r => ⟨[regex r w s cap, capture n s], []⟩
     | .backref d n => ⟨[regex (match (cap n).head? with
       | none => match d with | .bot => [/⊥/] | .empty => [//]
-      | some (cs, ct) => list (w.extract cs.val ct.val)
-      ) s cap], []⟩
-  | .concatWait _ r _ => ⟨if h : arg = []
+      | some (cs, ct) => list (w.extract cs ct)
+      ) w s cap], []⟩
+  | .concatWait _ r w _ => ⟨if h : arg = []
     then []
-    else [concat r ((arg.map Prod.fst).min
+    else [concat r w ((arg.map Prod.fst).min
       (by contrapose! h; exact List.map_eq_nil_iff.mp h)) arg []], []⟩
-  | .concat r s old new => match old with
+  | .concat r w s old new => match old with
     | [] => ⟨[], new ++ arg⟩
-    | (s', cap) :: old => ⟨[regex r s' cap, concat r s old (new ++ arg)], []⟩
-  | .orWait r s cap => ⟨[regex r s cap, or s arg], []⟩
+    | (s', cap) :: old => ⟨[regex r w s' cap, concat r w s old (new ++ arg)], []⟩
+  | .orWait r w s cap => ⟨[regex r w s cap, or s arg], []⟩
   | .or _ fst => ⟨[], fst ++ arg⟩
   | .filterEmpty emp s => ⟨[], arg.filter fun (s', _) ↦ (s ≥ s') = emp⟩
   | .capture n s => ⟨[], arg.map fun (s', cap) ↦
       (s', cap.update n [(s, s')])⟩
 
 /-- The position associated with an action. Used for position lawfulness proofs -/
-def Action.pos (ac : Action w) : Pos w := match ac with
-  | .regex _ s _ => s
-  | .concatWait _ _ s => s
-  | .concat _ s _ _ => s
-  | .orWait _ s _ => s
+def Action.pos (ac : Action α) : ℕ := match ac with
+  | .regex _ _ s _ => s
+  | .concatWait _ _ _ s => s
+  | .concat _ _ s _ _ => s
+  | .orWait _ _ s _ => s
   | .or s _ => s
   | .filterEmpty _ s => s
   | .capture _ s => s
 
+-- Apparently without the dependent argument `w`, the type checker doesn't
+-- realize that `StepResult α` is a monad on `MatchStack α` and won't
+-- let `bind` through
+
 /-- The result of stepping the match stack. Either the next state or the
 match result -/
-def StepResult (w : List α) := Except (PartialMatches w) (MatchStack w)
+def StepResult := Except PartialMatches
+  deriving Monad, LawfulMonad
 
 /-- Constructs a match stack out of a single action -/
-def Action.matchStack (ac : Action w) (arg : PartialMatches w)
-    : MatchStack w := MatchStack.mk [ac] arg
+def Action.matchStack (ac : Action α) (arg : PartialMatches)
+    : MatchStack α := MatchStack.mk [ac] arg
 
 namespace MatchStack
 
 /-- Advancing the state of the regex matches. The state steps successfully
 unless the stack is empty, in which case the list of matches is returned -/
-def step (st : MatchStack w) : StepResult w
+def step (st : MatchStack α) : StepResult (MatchStack α)
   := match st.entries with
   | [] => Except.error st.arg
   | action :: stack => let ⟨entries, return'⟩ := action.process st.arg
     Except.ok ⟨entries ++ stack, return'⟩
 
-theorem step_eq_ok {st st' : MatchStack w} (hst : st.step = Except.ok st')
-    : ∃ (ac : Action w) (as : List (Action w)), st.entries = ac :: as ∧ st' = MatchStack.mk
+theorem step_eq_ok {st st' : MatchStack α} (hst : st.step = Except.ok st')
+    : ∃ (ac : Action α) (as : List (Action α)), st.entries = ac :: as ∧ st' = MatchStack.mk
         (entries := (ac.process st.arg).entries ++ as)
         (arg := (ac.process st.arg).arg)
         := by
@@ -99,19 +104,19 @@ theorem step_eq_ok {st st' : MatchStack w} (hst : st.step = Except.ok st')
   rw [Except.ok.injEq] at hst
   exact ⟨ac, as', has, Eq.symm hst⟩
 
-theorem step_eq_error {st : MatchStack w} {mat : PartialMatches w}
+theorem step_eq_error {st : MatchStack α} {mat : PartialMatches}
     (hst : st.step = Except.error mat)
     : st.entries = [] := by
   rw [step] at hst; split at hst <;> first | assumption | simp at hst
 
-theorem step_eq_error_iff {st : MatchStack w}
+theorem step_eq_error_iff {st : MatchStack α}
     : st.step = Except.error st.arg ↔ st.entries = [] := by
   constructor
   · exact fun hst ↦ st.step_eq_error hst
   · intro hst
     rw [step, hst]
 
-theorem step_singleton (ac : Action w) (arg : PartialMatches w)
+theorem step_singleton (ac : Action α) (arg : PartialMatches)
     : (MatchStack.mk [ac] arg).step = Except.ok (ac.process arg) := by
   simp [step]
 
