Regex/Basic.lean
@@ -11,7 +11,7 @@ import Regex.Util
 namespace Regex
 
 variable {α : Type u} [deq : DecidableEq α] {r : Regex α} {w : List α}
-  {s : Pos w} {cap : Captures w}
+  {s : ℕ} {cap : Captures}
 
 theorem StarType.map_match {α β : Type*} (f : α → β) (t : StarType) (g l : α)
     : f (match t with | .greedy => g | .lazy => l) =
@@ -24,13 +24,13 @@ theorem StarType.flatten_match {α : Type*} (t : StarType) (gg gl lg ll : α)
       (match t with | .greedy => gg | .lazy => ll) := by rcases t <;> simp
 
 /-- Initialize a partial match stack -/
-def initMatchPartial (r : Regex α) (w : List α) (s : Pos w) (cap : Captures w)
-    : MatchStack w where
-  entries := [Action.regex r s cap]
+def initMatchPartial (r : Regex α) (w : List α) (s : ℕ) (cap : Captures)
+    : MatchStack α where
+  entries := [Action.regex r w s cap]
   arg := []
 
 /-- Whether a particular regex match terminates -/
-def Terminates (r : Regex α) (w : List α) (s : Pos w) (cap : Captures w) :=
+def Terminates (r : Regex α) (w : List α) (s : ℕ) (cap : Captures) :=
   (r.initMatchPartial w s cap).Terminates
 
 /-! Some tactics for proving termination -/
@@ -178,35 +178,35 @@ end Tactic
 section MatchPartial
 open MatchStack
 
-def matchPartial (r : Regex α) (w : List α) (s : Pos w) (cap : Captures w)
+def matchPartial (r : Regex α) (w : List α) (s : ℕ) (cap : Captures)
   (term : r.Terminates w s cap)
-    : PartialMatches w := (r.initMatchPartial w s cap).run term
+    : PartialMatches := (r.initMatchPartial w s cap).run term
 
-theorem matchPartial_terminates_iff {r : Regex α} {w : List α} {s : Pos w} {cap : Captures w}
-    : r.Terminates w s cap ↔ (mk [.regex r s cap] []).Terminates := iff_of_eq rfl
+theorem matchPartial_terminates_iff
+    : r.Terminates w s cap ↔ (mk [.regex r w s cap] []).Terminates := iff_of_eq rfl
 
-theorem matchPartial_eq_run {r : Regex α} {w : List α} {s : Pos w} {cap : Captures w}
+theorem matchPartial_eq_run
   {term : r.Terminates w s cap}
-    : r.matchPartial w s cap term = (mk [.regex r s cap] []).run term := rfl
+    : r.matchPartial w s cap term = (mk [.regex r w s cap] []).run term := rfl
 
 /-- `bot` always terminates -/
-theorem bot_terminates {s : Pos w} {cap : Captures w}
+theorem bot_terminates
     : [/⊥/].Terminates w s cap := by
   rw [Terminates, initMatchPartial]; step; step
 
 /-- `empty` always terminates -/
-theorem empty_terminates {s : Pos w} {cap : Captures w}
+theorem empty_terminates
     : [//].Terminates w s cap := by
   rw [Terminates, initMatchPartial]; step; step
 
 /-- `unit` always terminates -/
-theorem unit_terminates {c : α} {s : Pos w} {cap : Captures w}
+theorem unit_terminates {c : α}
     : [/c/].Terminates w s cap := by
   rw [Terminates, initMatchPartial]; step; step
 
-theorem Action.concat_terminates {r : Regex α} {s : Pos w}
-    {old new arg : PartialMatches w}
-    : (MatchStack.mk [concat r s old new] arg).Terminates ↔
+theorem Action.concat_terminates
+    {old new arg : PartialMatches}
+    : (MatchStack.mk [concat r w s old new] arg).Terminates ↔
       ∀ mat ∈ old, r.Terminates w mat.1 mat.2 := by
   constructor
   · intro term mat mem
@@ -224,8 +224,8 @@ theorem Action.concat_terminates {r : Regex α} {s : Pos w}
       use term ent List.mem_cons_self
       exact ind fun m mem ↦ term _ (List.mem_cons_of_mem _ mem)
 
-theorem Action.concatWait_terminates {q r : Regex α} {s : Pos w} {arg : PartialMatches w}
-    : (MatchStack.mk [concatWait q r s] arg).Terminates ↔
+theorem Action.concatWait_terminates {q r : Regex α} {arg : PartialMatches}
+    : (MatchStack.mk [concatWait q r w s] arg).Terminates ↔
       ∀ mat ∈ arg, r.Terminates w mat.1 mat.2 := by
   constructor
   · intro term mat mem
@@ -242,7 +242,7 @@ theorem Action.concatWait_terminates {q r : Regex α} {s : Pos w} {arg : Partial
 
 /-- `concat q r` terminates iff `q` terminates and `r` terminates for every
 end position and match provided by `q` -/
-theorem concat_terminates {q r : Regex α} {s : Pos w} {cap : Captures w}
+theorem concat_terminates {q r : Regex α}
     : [/⟨q⟩ ⟨r⟩/].Terminates w s cap ↔ (term : q.Terminates w s cap) ∧
       ∀ mat ∈ q.matchPartial w s cap term, r.Terminates w mat.1 mat.2 := by
   constructor
@@ -262,12 +262,12 @@ theorem concat_terminates {q r : Regex α} {s : Pos w} {cap : Captures w}
     rw [Action.concatWait_terminates]
     exact fun mat run ↦ term mat run
 
-theorem Action.or_terminates {s : Pos w} {fst arg : PartialMatches w}
-    : (MatchStack.mk [or s fst] arg).Terminates := by step; step
+theorem Action.or_terminates {fst arg : PartialMatches}
+    : (MatchStack.mk [or (α := α) s fst] arg).Terminates := by step; step
 
-theorem Action.orWait_terminates {r : Regex α} {s : Pos w} {cap : Captures w}
-    {arg : PartialMatches w}
-    : (MatchStack.mk [orWait r s cap] arg).Terminates ↔ r.Terminates w s cap := by
+theorem Action.orWait_terminates
+    {arg : PartialMatches}
+    : (MatchStack.mk [orWait r w s cap] arg).Terminates ↔ r.Terminates w s cap := by
   constructor
   · intro term
     step at term
@@ -279,7 +279,7 @@ theorem Action.orWait_terminates {r : Regex α} {s : Pos w} {cap : Captures w}
     exact or_terminates
 
 /-- `or q r` terminates iff `q` terminates and `r` terminates -/
-theorem or_terminates {q r : Regex α} {s : Pos w} {cap : Captures w}
+theorem or_terminates {q r : Regex α}
     : [/⟨q⟩ | ⟨r⟩/].Terminates w s cap ↔
       q.Terminates w s cap ∧ r.Terminates w s cap := by
   constructor
@@ -294,12 +294,11 @@ theorem or_terminates {q r : Regex α} {s : Pos w} {cap : Captures w}
     run_top! using qterm
     exact Action.orWait_terminates.mpr rterm
 
-theorem Action.filterEmpty_terminates {emp : Bool} {s : Pos w} {arg : PartialMatches w}
-    : (MatchStack.mk [filterEmpty emp s] arg).Terminates := by step; step
+theorem Action.filterEmpty_terminates {emp : Bool} {arg : PartialMatches}
+    : (MatchStack.mk [filterEmpty (α := α) emp s] arg).Terminates := by step; step
 
 /-- `filterEmpty emp r` terminates iff `r` terminates -/
-theorem filterEmpty_terminates {emp : Bool} {r : Regex α}
-    {s : Pos w} {cap : Captures w}
+theorem filterEmpty_terminates {emp : Bool}
     : [/⟨r⟩ ‹emp›ε/].Terminates w s cap ↔ r.Terminates w s cap := by
   constructor <;> intro term
   · rw [Terminates, initMatchPartial] at term
@@ -312,19 +311,18 @@ theorem filterEmpty_terminates {emp : Bool} {r : Regex α}
     exact ⟨term, Action.filterEmpty_terminates⟩
 
 /-- `start` always terminates -/
-theorem start_terminates {s : Pos w} {cap : Captures w}
+theorem start_terminates
     : [/⊢/].Terminates w s cap := by rw [Terminates, initMatchPartial]; step; step
 
 /-- `end'` always terminates -/
-theorem end'_terminates {s : Pos w} {cap : Captures w}
+theorem end'_terminates
     : [/⊣/].Terminates w s cap := by rw [Terminates, initMatchPartial]; step; step
 
-theorem Action.capture_terminates {n : ℕ} {s : Pos w} {arg : PartialMatches w}
-    : (MatchStack.mk [capture n s] arg).Terminates := by step; step
+theorem Action.capture_terminates {n : ℕ} {arg : PartialMatches}
+    : (MatchStack.mk [capture (α := α) n s] arg).Terminates := by step; step
 
 /-- `capture emp r` terminates iff `r` terminates -/
-theorem capture_terminates {n : ℕ} {r : Regex α}
-    {s : Pos w} {cap : Captures w}
+theorem capture_terminates {n : ℕ}
     : [/(‹n› ⟨r⟩)/].Terminates w s cap ↔ r.Terminates w s cap := by
   constructor <;> intro term
   · rw [Terminates, initMatchPartial] at term
@@ -336,23 +334,23 @@ theorem capture_terminates {n : ℕ} {r : Regex α}
     run_top!
     exact ⟨term, Action.capture_terminates⟩
 
-theorem matchPartial_bot (s : Pos w) (cap : Captures w)
+theorem matchPartial_bot
     : matchPartial [/⊥/] w s cap bot_terminates = [] := by
   simp only [matchPartial_eq_run]; step; step
 
-theorem matchPartial_empty (s : Pos w) (cap : Captures w)
+theorem matchPartial_empty
     : matchPartial [//] w s cap empty_terminates
     = [(s, cap)] := by
   simp only [matchPartial_eq_run]; step; step
 
-theorem matchPartial_unit (c : α) (s : Pos w) (cap : Captures w)
+theorem matchPartial_unit {c : α}
     : matchPartial [/c/] w s cap unit_terminates
-      = if h : w[s.val]? = some c then [(s.succOfIndex h, cap)] else [] := by
+      = if w[s]? = some c then [(s + 1, cap)] else [] := by
   simp only [matchPartial_eq_run]; step; step
 
-theorem Action.concat_run {r : Regex α} {s : Pos w} {old new arg : PartialMatches w}
+theorem Action.concat_run {old new arg : PartialMatches}
     (term : ∀ mat ∈ old, r.Terminates w mat.1 mat.2)
-    : (mk [.concat r s old new] arg).run (concat_terminates.mpr term)
+    : (mk [.concat r w s old new] arg).run (concat_terminates.mpr term)
       = new ++ arg ++
       (old.pmap (fun ent rt ↦ r.matchPartial w ent.1 ent.2 rt) term).flatten := by
   induction old generalizing new arg with | nil => step; step | cons ent mat ind =>
@@ -365,9 +363,9 @@ theorem Action.concat_run {r : Regex α} {s : Pos w} {old new arg : PartialMatch
       List.append_cancel_right_eq]
     rfl
 
-theorem Action.concatWait_run {q r : Regex α} {s : Pos w} {arg : PartialMatches w}
+theorem Action.concatWait_run {q r : Regex α} {arg : PartialMatches}
     (term : ∀ mat ∈ arg, r.Terminates w mat.1 mat.2)
-    : (mk [.concatWait q r s] arg).run (concatWait_terminates.mpr term)
+    : (mk [.concatWait q r w s] arg).run (concatWait_terminates.mpr term)
       = (arg.pmap (fun ent rt ↦ r.matchPartial w ent.1 ent.2 rt) term).flatten := by
   step
   cases arg with | nil => step | cons ent mat =>
@@ -375,8 +373,8 @@ theorem Action.concatWait_run {q r : Regex α} {s : Pos w} {arg : PartialMatches
       List.flatten_cons]
     simp [concat_run term]
 
-theorem matchPartial_concat (q r : Regex α) (s : Pos w) (cap : Captures w)
-    (term : [/⟨q⟩ ⟨r⟩/].Terminates w s cap)
+theorem matchPartial_concat (q r : Regex α) (s : ℕ) (cap : Captures)
+    {term : [/⟨q⟩ ⟨r⟩/].Terminates w s cap}
     : matchPartial [/⟨q⟩ ⟨r⟩/] w s cap term
       = ((q.matchPartial w s cap (concat_terminates.mp term).1).pmap
           (fun ent rt ↦ r.matchPartial w ent.1 ent.2 rt)
@@ -388,16 +386,16 @@ theorem matchPartial_concat (q r : Regex α) (s : Pos w) (cap : Captures w)
   rw! [← matchPartial_eq_run]
   rw [Action.concatWait_run (concat_terminates.mp term).2]
 
-theorem Action.or_run {s : Pos w} {fst arg : PartialMatches w}
-    : (mk [.or s fst] arg).run or_terminates = fst ++ arg := by step; step
+theorem Action.or_run {s : ℕ} {fst arg : PartialMatches}
+    : (mk [.or (α := α) s fst] arg).run or_terminates = fst ++ arg := by step; step
 
-theorem Action.orWait_run {r : Regex α} {s : Pos w} {cap : Captures w}
-    {arg : PartialMatches w} (term : r.Terminates w s cap)
-    : (mk [.orWait r s cap] arg).run (orWait_terminates.mpr term)
+theorem Action.orWait_run {r : Regex α} {s : ℕ} {cap : Captures}
+    {arg : PartialMatches} (term : r.Terminates w s cap)
+    : (mk [.orWait r w s cap] arg).run (orWait_terminates.mpr term)
       = arg ++ r.matchPartial w s cap term := by step; run_top!; step; step; rfl
 
-theorem matchPartial_or (q r : Regex α) (s : Pos w) (cap : Captures w)
-    (term : [/⟨q⟩ | ⟨r⟩/].Terminates w s cap)
+theorem matchPartial_or {q r : Regex α}
+    {term : [/⟨q⟩ | ⟨r⟩/].Terminates w s cap}
     : matchPartial [/⟨q⟩ | ⟨r⟩/] w s cap term
       = q.matchPartial w s cap (or_terminates.mp term).1 ++
         r.matchPartial w s cap (or_terminates.mp term).2 := by
@@ -408,12 +406,12 @@ theorem matchPartial_or (q r : Regex α) (s : Pos w) (cap : Captures w)
   rw [Action.orWait_run (or_terminates.mp term).2]
   rfl
 
-theorem Action.filterEmpty_run {emp : Bool} {s : Pos w} {arg : PartialMatches w}
-    : (mk [.filterEmpty emp s] arg).run filterEmpty_terminates
+theorem Action.filterEmpty_run {emp : Bool} {arg : PartialMatches}
+    : (mk [.filterEmpty (α := α) emp s] arg).run filterEmpty_terminates
       = arg.filter fun ent => (s ≥ ent.1) = emp := by step; step
 
-theorem matchPartial_filterEmpty (emp : Bool) (r : Regex α) (s : Pos w) (cap : Captures w)
-    (term : [/⟨r⟩ ‹emp›ε/].Terminates w s cap)
+theorem matchPartial_filterEmpty (emp : Bool)
+    {term : [/⟨r⟩ ‹emp›ε/].Terminates w s cap}
     : matchPartial [/⟨r⟩ ‹emp›ε/] w s cap term =
       (r.matchPartial w s cap (filterEmpty_terminates.mp term)).filter
         fun ent ↦ (s ≥ ent.1) = emp := by
@@ -424,20 +422,17 @@ theorem matchPartial_filterEmpty (emp : Bool) (r : Regex α) (s : Pos w) (cap : 
   simp only [Action.filterEmpty_run, eq_iff_iff, Bool.decide_iff_dist, Bool.decide_eq_true]
   rfl
 
-theorem matchPartial_star_greedy_terminates' {r : Regex α} {s : Pos w}
-    {cap : Captures w}
+theorem matchPartial_star_greedy_terminates'
     : [/⟨r⟩*/].Terminates w s cap ↔
       [/(⟨r⟩ •ε | (⟨r⟩ -ε) ⟨r⟩*) | ε/].Terminates w s cap := by
   simp only [Terminates, initMatchPartial]; conv_lhs => step
 
-theorem matchPartial_star_lazy_terminates' {r : Regex α} {s : Pos w}
-    {cap : Captures w}
+theorem matchPartial_star_lazy_terminates'
     : [/⟨r⟩*?/].Terminates w s cap ↔
       [/ε | (⟨r⟩ •ε | (⟨r⟩ -ε) ⟨r⟩*?)/].Terminates w s cap := by
   simp only [Terminates, initMatchPartial]; conv_lhs => step
 
-theorem star_terminates' {t : StarType} {r : Regex α} {s : Pos w}
-    {cap : Captures w}
+theorem star_terminates' {t : StarType}
     : [/⟨r⟩*‹t›/].Terminates w s cap ↔ match t with
       | .greedy => [/(⟨r⟩ •ε | (⟨r⟩ -ε) ⟨r⟩*) | ε/].Terminates w s cap
       | .lazy => [/ε | (⟨r⟩ •ε | (⟨r⟩ -ε) ⟨r⟩*?)/].Terminates w s cap := by
@@ -449,8 +444,7 @@ theorem star_terminates' {t : StarType} {r : Regex α} {s : Pos w}
 
 /-- `star t r` terminates iff `r` terminates and `r` terminates for every
 advancing end position and match provided by `r` -/
-theorem star_terminates {t : StarType} {r : Regex α} {s : Pos w}
-    {cap : Captures w}
+theorem star_terminates {t : StarType}
     : [/⟨r⟩*‹t›/].Terminates w s cap ↔ (term : r.Terminates w s cap) ∧
       ∀ mat ∈ r.matchPartial w s cap term,
         s < mat.1 → [/⟨r⟩*‹t›/].Terminates w mat.1 mat.2 := by
@@ -472,22 +466,7 @@ theorem star_terminates {t : StarType} {r : Regex α} {s : Pos w}
       filterEmpty_terminates]
     simp [dand_iff_and_forall, empty_terminates, matchPartial_filterEmpty]
 
-/-- `star t r` terminates if (but not only if)
-`r` terminates for every capture and for every position starting from here -/
-theorem star_terminates_of_forall {t : StarType} {r : Regex α} {s : Pos w}
-    {cap : Captures w}
-    : (∀ s' ≥ s, ∀ cap', r.Terminates w s' cap') →
-      [/⟨r⟩*‹t›/].Terminates w s cap := by
-  intro term
-  induction h : s.distToEnd using Nat.strongRec generalizing s cap with
-  | ind n ind =>
-    rw [star_terminates]
-    refine ⟨term s (le_refl _) cap, fun mat mem lt ↦ ?_⟩
-    simp only [← h] at ind
-    exact ind mat.1.distToEnd (Icc.distToEnd_lt.mp lt)
-      (fun s' ge ↦ term s' (le_of_lt (Trans.trans lt ge))) rfl
-
-theorem matchPartial_star (t : StarType) (r : Regex α) (s : Pos w) (cap : Captures w)
+theorem matchPartial_star {t : StarType}
     (term : [/⟨r⟩*‹t›/].Terminates w s cap)
     : matchPartial [/⟨r⟩*‹t›/] w s cap term = match t with
       | .greedy => [/(⟨r⟩ •ε | (⟨r⟩ -ε) ⟨r⟩*) | ε/].matchPartial w s cap
@@ -498,21 +477,21 @@ theorem matchPartial_star (t : StarType) (r : Regex α) (s : Pos w) (cap : Captu
   simp only [matchPartial_eq_run]
   split <;> conv_lhs => step
 
-theorem matchPartial_start (s : Pos w) (cap : Captures w)
+theorem matchPartial_start
     : matchPartial [/⊢/] w s cap start_terminates
       = if s = 0 then [(s, cap)] else [] := by
   simp only [matchPartial_eq_run]; step; step
 
-theorem matchPartial_end' (s : Pos w) (cap : Captures w)
+theorem matchPartial_end'
     : matchPartial [/⊣/] w s cap end'_terminates
-      = if s = s.end' then [(s, cap)] else [] := by
+      = if s = w.length then [(s, cap)] else [] := by
   simp only [matchPartial_eq_run]; step; step
 
-theorem Action.capture_run {n : ℕ} {s : Pos w} {arg : PartialMatches w}
-    : (mk [.capture n s] arg).run capture_terminates
+theorem Action.capture_run {n : ℕ} {arg : PartialMatches}
+    : (mk [.capture (α := α) n s] arg).run capture_terminates
       = arg.map fun ent ↦ (ent.1, ent.2.update n [(s, ent.1)]) := by step; step
 
-theorem matchPartial_capture (n : ℕ) (r : Regex α) (s : Pos w) (cap : Captures w)
+theorem matchPartial_capture {n : ℕ}
     (term : [/(‹n› ⟨r⟩)/].Terminates w s cap)
     : matchPartial [/(‹n› ⟨r⟩)/] w s cap term =
       (r.matchPartial w s cap (capture_terminates.mp term)).map
@@ -525,20 +504,19 @@ theorem matchPartial_capture (n : ℕ) (r : Regex α) (s : Pos w) (cap : Capture
   rfl
 
 /-- `list` always terminates -/
-theorem list_terminates {l : List α} {s : Pos w} {cap : Captures w}
+theorem list_terminates {l : List α}
     : (list l).Terminates w s cap := by
   induction l generalizing s with
   | nil => rw [list]; exact empty_terminates
   | cons a as ind =>
     rw [list, concat_terminates]
-    simp only [matchPartial_unit, List.mem_dite_nil_right, List.mem_cons,
-      List.not_mem_nil, or_false, forall_exists_index, forall_eq_apply_imp_iff,
-      dand_iff_and_forall, unit_terminates, forall_const, true_and]
+    simp only [matchPartial_unit, List.mem_ite_nil_right, List.mem_cons, List.not_mem_nil, or_false,
+      and_imp, forall_eq_apply_imp_iff, dand_iff_and_forall, unit_terminates, forall_const,
+      true_and]
     exact fun _ ↦ ind
 
 /-- `backref` always terminates -/
 theorem backref_terminates {d : BackrefDefault} {n : ℕ}
-    {s : Pos w} {cap : Captures w}
     : [/\‹d›n/].Terminates w s cap := by
   rw [matchPartial_terminates_iff]
   step
@@ -546,48 +524,42 @@ theorem backref_terminates {d : BackrefDefault} {n : ℕ}
   · split <;> (step; step)
   exact list_terminates
 
-theorem matchPartial_list (l : List α) (s : Pos w) (cap : Captures w)
+theorem matchPartial_list {l : List α}
     : matchPartial (list l) w s cap list_terminates =
-    if h : w.extract s.val (s.val + l.length) = l
-      then [(s.addOfIndex h rfl, cap)] else [] := by
+    if w.extract s (s + l.length) = l then [(s + l.length, cap)] else [] := by
   induction l generalizing s with
-  | nil => simp [list, matchPartial_empty, Icc.addOfIndex]
+  | nil => simp [list, matchPartial_empty]
   | cons a as ind =>
     simp only [list, matchPartial_concat, List.length_cons, matchPartial_unit]
-    by_cases! h : w[s.val]? = a
-    · specialize ind (s.succOfIndex h)
-      simp only [h, ↓reduceDIte, List.pmap_cons, ind, Icc.succOfIndex_val,
+    by_cases! h : w[s]? = a
+    · specialize ind (s := s + 1)
+      simp only [h, ↓reduceIte, List.pmap_cons, ind,
         List.pmap_nil, List.flatten_cons, List.flatten_nil, List.append_nil]
       rw! [← add_assoc, add_right_comm]
-      have eq : (w.extract (s.val + 1) (s.val + as.length + 1) = as)
-          = (w.extract (s.val) (s.val + as.length + 1) = a :: as) := by
+      have eq : (w.extract (s + 1) (s + as.length + 1) = as)
+          = (w.extract (s) (s + as.length + 1) = a :: as) := by
         simp only [List.extract_eq_drop_take, Nat.reduceSubDiff, add_tsub_cancel_left,
-        eq_iff_iff]
+          eq_iff_iff]
         rw [add_assoc, Nat.add_sub_cancel_left]
         have ⟨lt, wsa⟩ := List.getElem?_eq_some_iff.mp h
         conv_rhs => rw [List.drop_eq_getElem_cons lt, List.take_cons (by linarith), wsa]
         simp
       simp only [eq]
-      split
-      · simp [← Icc.val_inj, add_assoc, add_comm 1]
-      · rfl
-    simp only [h, ↓reduceDIte, List.pmap_nil, List.flatten_nil, List.extract_eq_drop_take,
-      right_eq_dite_iff, List.ne_cons_self, imp_false]
-    by_cases! h' : s.val < w.length
+    simp only [h, ↓reduceIte, List.pmap_nil, List.flatten_nil, List.extract_eq_drop_take,
+      add_tsub_cancel_left, right_eq_ite_iff, List.ne_cons_self, imp_false]
+    by_cases! h' : s < w.length
     · contrapose! h
-      rw [Nat.add_sub_cancel_left, List.drop_eq_getElem_cons h',
-        List.take_cons (by linarith)] at h
+      rw [List.drop_eq_getElem_cons h', List.take_cons (by linarith)] at h
       simp only [add_tsub_cancel_right, List.cons.injEq] at h
       rw [← h.1, List.getElem?_eq_some_getElem_iff]; trivial
     · simp [List.drop_eq_nil_of_le h']
 
-theorem matchPartial_backref (d : BackrefDefault) (n : ℕ) (s : Pos w) (cap : Captures w)
+theorem matchPartial_backref {n : ℕ} {d : BackrefDefault}
     : matchPartial [/\‹d›n/] w s cap backref_terminates =
       match (cap n).head? with
       | none => match d with | .bot => [] | .empty => [(s, cap)]
-      | some (cs, ct) => if h : w.extract s.val (s.val + (ct.val - cs.val))
-          = w.extract cs.val ct.val
-        then [(s.addOfIndex h (List.length_extract_nat' cs.is_le ct.is_le), cap)]
+      | some (cs, ct) => if w.extract s (s + (w.extract cs ct).length) = w.extract cs ct
+        then [(s + (w.extract cs ct).length, cap)]
         else [] := by
   rw [matchPartial_eq_run]
   step only [List.append_nil]
@@ -597,8 +569,7 @@ theorem matchPartial_backref (d : BackrefDefault) (n : ℕ) (s : Pos w) (cap : C
   · simp only [← heeq, h]
     split <;> (step; step)
   · simp only [← heeq, h]
-    rw! [← matchPartial_eq_run, matchPartial_list,
-      List.length_extract_nat' val.1.is_le val.2.is_le]
+    rw! [← matchPartial_eq_run, matchPartial_list]
     rfl
 
 end MatchPartial
@@ -618,11 +589,11 @@ end Tactic
 
 /-- Returns all matches that end at the end of the string -/
 def match' (r : Regex α) (w : List α) (term : r.Terminates w 0 0) :
-  PartialMatches w := [/⟨r⟩ ⊣/].matchPartial w 0 0
+  PartialMatches := [/⟨r⟩ ⊣/].matchPartial w 0 0
     (concat_terminates.mpr ⟨term, fun _ _ ↦ end'_terminates⟩)
 
 theorem match'_def {r : Regex α} {w : List α} (term : r.Terminates w 0 0)
-    : r.match' w term = (r.matchPartial w 0 0 term).filter fun mat ↦ mat.1 = mat.1.end' := by
+    : r.match' w term = (r.matchPartial w 0 0 term).filter fun mat ↦ mat.1 = w.length := by
   rw [match', matchPartial_concat]
   simp only [matchPartial_end', Prod.mk.eta, List.pmap_eq_map]
   rw [← List.flatMap_def, ← List.filterMap_eq_filter, List.filterMap_eq_flatMap_toList]
@@ -640,16 +611,15 @@ theorem isMatch_bot : ¬[/⊥/].isMatch w bot_terminates := by
 
 /-- The empty regex matches only the empty string -/
 theorem isMatch_empty : [//].isMatch w empty_terminates ↔ w = [] := by
-  simp [isMatch, match'_def, matchPartial_empty]
-  simp [Icc.zero_end']
+  simp only [isMatch, match'_def, matchPartial_empty, List.isEmpty_iff, List.filter_eq_nil_iff,
+    List.mem_cons, List.not_mem_nil, or_false, decide_eq_true_eq, forall_eq, Decidable.not_not]
+  rw [eq_comm, List.length_eq_zero_iff]
 
 /-- A unit regex matches only the singleton sequence that has that unit -/
 theorem isMatch_unit {c : α} : [/`‹c›/].isMatch w unit_terminates ↔ w = [c] := by
-  simp only [isMatch, match'_def, ← Icc.val_inj, Icc.end'_val, matchPartial_unit,
-    Icc.zero_val, List.isEmpty_iff, List.filter_eq_nil_iff, List.mem_dite_nil_right,
-    List.mem_cons, List.not_mem_nil, or_false, decide_eq_true_eq, forall_exists_index,
-    forall_eq_apply_imp_iff, Icc.succOfIndex_val, zero_add, Classical.not_imp,
-    Decidable.not_not]
+  simp only [isMatch, match'_def, matchPartial_unit, zero_add, List.isEmpty_iff,
+    List.filter_eq_nil_iff, List.mem_ite_nil_right, List.mem_cons, List.not_mem_nil, or_false,
+    decide_eq_true_eq, and_imp, forall_eq_apply_imp_iff, Classical.not_imp, Decidable.not_not]
   rw [eq_comm (a := 1), List.length_eq_one_iff, List.getElem?_eq_some_iff]
   constructor
   · rintro ⟨⟨lt, eqc⟩, ⟨c', eqc'⟩⟩
@@ -670,20 +640,23 @@ theorem isMatch_filterEmpty {e : Bool} {r : Regex α}
     (term : [/⟨r⟩ ‹e›ε/].Terminates w 0 0)
     : [/⟨r⟩ ‹e›ε/].isMatch w term ↔
       r.isMatch w (filterEmpty_terminates.mp term) ∧ (w.length = 0) = e := by
-  simp [isMatch, match'_def, matchPartial_filterEmpty,
-    decide_eq_bool, Icc.end'_eq 0, Icc.val_le_val]
+  simp [isMatch, match'_def, matchPartial_filterEmpty, decide_eq_bool]
 
 -- Some silly ones
 
 /-- The start anchor full-matches only the empty sequence -/
 theorem isMatch_start : [/⊢/].isMatch w start_terminates ↔ w = [] := by
-  simp [isMatch, match'_def, matchPartial_start]
-  simp [Icc.zero_end']
+  simp only [isMatch, match'_def, matchPartial_start, ↓reduceIte, List.isEmpty_iff,
+    List.filter_eq_nil_iff, List.mem_cons, List.not_mem_nil, or_false, decide_eq_true_eq, forall_eq,
+    Decidable.not_not]
+  rw [eq_comm, List.length_eq_zero_iff]
 
 /-- The end anchor full-matches only the empty sequence -/
 theorem isMatch_end' : [/⊣/].isMatch w end'_terminates ↔ w = [] := by
-  simp [isMatch, match'_def, matchPartial_end']
-  simp [Icc.zero_end']
+  simp only [isMatch, match'_def, matchPartial_end', List.isEmpty_iff, List.filter_eq_nil_iff,
+    List.mem_ite_nil_right, List.mem_cons, List.not_mem_nil, or_false, decide_eq_true_eq, and_imp,
+    forall_eq_apply_imp_iff, imp_not_self, Decidable.not_not]
+  rw [eq_comm, List.length_eq_zero_iff]
 
 /-- A capture of `r` matches iff `r` matches -/
 theorem isMatch_capture {n : ℕ} {r : Regex α} (term : [/(‹n› ⟨r⟩)/].Terminates w 0 0)
@@ -696,7 +669,7 @@ theorem isMatch_backref {d : BackrefDefault} {n : ℕ}
         | .bot => False
         | .empty => w = [] := by
   simp [isMatch, match'_def, matchPartial_backref]
-  split <;> simp [Icc.zero_end']
+  split <;> simp
 
 def language (r : Regex α) (term : ∀ w, r.Terminates w 0 0)
   : Language α := {w | isMatch r w (term w)}
