Regex/PosCaptures.lean
@@ -10,386 +10,388 @@ namespace Regex
 
 variable {α : Type u} [deq : DecidableEq α] {w : List α}
 
-/-- Probably easier to work with than `Fin` and subtyping at the same time.
-`Icc a b` is the subtype of natural numbers `n` where `a ≤ n ≤ b`. -/
-def Icc (a b : ℕ) := {x : ℕ // a ≤ x ∧ x ≤ b}
-  deriving LE, LT, DecidableEq, Repr, Min, Max, LinearOrder,
-    Std.LawfulOrderMin, Std.LawfulOrderMax
-instance Icc.decLt {a b : ℕ} (i j : Icc a b) : Decidable (LT.lt i j) := Nat.decLt ..
-instance Icc.decLe {a b : ℕ} (i j : Icc a b) : Decidable (LE.le i j) := Nat.decLe ..
+-- No more Icc. Too much dependent type hell.
 
-section Icc
-
-variable {a b : ℕ}
-
-/-- A valid position in a string `w` (including the end) -/
-@[reducible] def Pos (w : List α) := Icc 0 w.length deriving Repr
-/-- A position from `c` to `b` -/
-@[reducible] def IccFrom (c : Icc a b) := Icc c.val b deriving Repr
-/-- A position from `a` to `c` -/
-@[reducible] def IccTo (c : Icc a b) := Icc a c.val deriving Repr
-
-namespace Icc
-
-theorem val_inj {s t : Icc a b} : s.val = t.val ↔ s = t := Subtype.val_inj
-theorem val_le_val {s t : Icc a b} : s ≤ t ↔ s.val ≤ t.val := by simp
-theorem val_lt_val {s t : Icc a b} : s < t ↔ s.val < t.val := by simp
-
-theorem is_ge (s : Icc a b) : a ≤ s.val := s.property.left
-theorem is_le (s : Icc a b) : s.val ≤ b := s.property.right
-
-end Icc
-
-omit deq in
-/-- The length of a list extraction using valid positions `s` and `t ≥ s`
-is just `t - s` with no underflow -/
-@[simp] theorem _root_.List.length_extract_icc (w : List α) (s : Pos w) (t : IccFrom s)
-    : (w.extract s.val t.val).length + s.val = t.val := by
-  simp only [List.extract_eq_drop_take, List.length_take, List.length_drop]
-  have mints : min (t.val - s.val) (w.length - s.val) = t.val - s.val := by
-    rw [min_eq_iff]
-    exact Or.inl ⟨rfl, (Nat.sub_le_sub_iff_right s.is_le).mpr t.is_le⟩
-  rw [mints, Nat.sub_add_cancel t.is_ge]
-
-omit deq in
-/-- The length of a list extraction using valid positions `s` and `t ≥ s`
-is just `t - s` with no underflow -/
-@[simp] theorem _root_.List.length_extract_nat {w : List α} {s t : ℕ}
-    (hs : s ≤ t) (ht : t ≤ w.length)
-    : (w.extract s t).length + s = t := by
-  let spos : Pos w := ⟨s, ⟨Nat.zero_le _, .trans hs ht⟩⟩
-  let tpos : IccFrom spos := ⟨t, ⟨hs, ht⟩⟩
-  have lex := List.length_extract_icc w spos tpos
-  simp only [spos, tpos] at lex
-  exact lex
-
---@[simp] theorem root_.List.min?_append (as bs : List α) (d : α)
---    : (as ++ bs).min? = as.m
-
-omit deq in
-/-- The length of a list extraction using valid positions `s` and `t`
-is just `t - s`, potentially with underflow -/
-@[simp] theorem _root_.List.length_extract_icc' (w : List α) (s : Pos w) (t : Pos w)
-    : (w.extract s.val t.val).length = t.val - s.val := by
-  simp only [List.extract_eq_drop_take, List.length_take, List.length_drop,
-    inf_eq_left, tsub_le_iff_right]
-  rw [Nat.sub_add_cancel s.prop.2]
-  exact t.prop.2
-
-omit deq in
-/-- The length of a list extraction using valid positions `s` and `t`
-is just `t - s`, potentially with underflow -/
-@[simp] theorem _root_.List.length_extract_nat' {w : List α} {s t : ℕ}
-    (hs : s ≤ w.length) (ht : t ≤ w.length)
-    : (w.extract s t).length = t - s :=
-  List.length_extract_icc' w ⟨s, ⟨Nat.zero_le _, hs⟩⟩ ⟨t, ⟨Nat.zero_le _, ht⟩⟩
-
-namespace Icc
-
-instance instZero : Zero (Icc 0 b) := ⟨0, ⟨le_refl 0, Nat.zero_le b⟩⟩
-
-@[simp] theorem zero_val : (0 : Icc 0 b).val = 0 := rfl
-
-/-- Turns `s` into a value bounded by itself and `b` -/
-def iccFrom (s : Icc a b) : IccFrom s := ⟨s.val, ⟨le_refl s.val, s.is_le⟩⟩
-
-/-- Turns `s` into a value bounded by `a` and itself -/
-def iccTo (s : Icc a b) : IccTo s := ⟨s.val, ⟨s.is_ge, le_refl s.val⟩⟩
-
-@[simp] theorem iccFrom_val (s : Icc a b) : s.iccFrom.val = s.val := rfl
-@[simp] theorem iccTo_val (s : Icc a b) : s.iccTo.val = s.val := rfl
-
-theorem le_of_mem_iccFrom {s t : Icc a b} {t' : IccFrom s} (ht : t.val = t'.val)
-    : s.val ≤ t.val := ht ▸ t'.is_ge
-
-theorem ne_of_lt_of_mem_iccFrom {s t : Icc a b} (t' : IccFrom s) (ht : t.val < s.val)
-    : t.val ≠ t'.val := by
-  contrapose! ht
-  exact le_of_mem_iccFrom ht
-
-/-- Expands the bounds of `s` -/
-def expand (s : Icc a b) {a' b' : ℕ} (ha : a' ≤ a) (hb : b ≤ b') : Icc a' b' :=
-  ⟨s.val, ⟨le_trans ha s.is_ge, le_trans s.is_le hb⟩⟩
-
-/-- Expands the lower bound of `s` -/
-def expandLeft (s : Icc a b) {a' : ℕ} (ha : a' ≤ a) : Icc a' b :=
-  s.expand ha (le_refl b)
-
-/-- Expands the upper bound of `s` -/
-def expandRight (s : Icc a b) {b' : ℕ} (hb : b ≤ b') : Icc a b' :=
-  s.expand (le_refl a) hb
-
-/-- Expands the lower bound of `s` to 0 -/
-def expandZero (s : Icc a b) : Icc 0 b := s.expandLeft (Nat.zero_le a)
-
-@[simp] theorem expand_val (s : Icc a b) {a' b' : ℕ} (ha : a' ≤ a) (hb : b ≤ b')
-    : (s.expand ha hb).val = s.val := by rfl
-
-@[simp] theorem expandZero_val (s : Icc a b)
-    : s.expandZero.val = s.val := by rfl
-
-@[simp] theorem expand_eq (s : Icc a b) : s.expand (le_refl a) (le_refl b) = s := rfl
-
-@[simp] theorem iccFrom_expandLeft (s : Icc a b) {a' : ℕ} (ha : a' ≤ a)
-    : IccFrom (s.expandLeft ha) = IccFrom s := rfl
-
-@[simp] theorem iccTo_expandRight (s : Icc a b) {b' : ℕ} (hb : b ≤ b')
-    : IccTo (s.expandRight hb) = IccTo s := rfl
-
-@[simp] theorem iccFrom_expandZero (s : Icc a b)
-    : IccFrom s.expandZero = IccFrom s := rfl
-
-/-- Use `s` to expand the lower bound of `s'` to the lower bound of `s` -/
-def widenLeft {s : Icc a b} (s' : IccFrom s) : Icc a b := s'.expandLeft s.is_ge
-
-/-- Use `s` to expand the upper bound of `s'` to the upper bound of `s` -/
-def widenRight {s : Icc a b} (s' : IccTo s) : Icc a b := s'.expandRight s.is_le
-
-def widenLeft' {s : Icc a b} (s' : IccFrom s) (a' : IccTo s) : Icc a'.val b :=
-  s'.expandLeft a'.is_le
-
-def widenRight' {s : Icc a b} (s' : IccTo s) (b' : IccFrom s) : Icc a b'.val :=
-  s'.expandRight b'.is_ge
-
-@[simp] theorem widenLeft_val {s : Icc a b} (s' : IccFrom s)
-    : (s.widenLeft s').val = s'.val := rfl
-
-@[simp] theorem widenRight_val {s : Icc a b} (s' : IccTo s)
-    : (s.widenRight s').val = s'.val := rfl
-
-@[simp] theorem widenLeft'_val {s : Icc a b} (s' : IccFrom s) (a' : IccTo s)
-    : (s.widenLeft' s' a').val = s'.val := rfl
-
-@[simp] theorem widenRight'_val {s : Icc a b} (s' : IccTo s) (b' : IccFrom s)
-    : (s.widenRight' s' b').val = s'.val := rfl
-
-/-- Given a subinterval to restrict positions `s` and `t` to, gives an new `s'` and `t'`
-for that subinterval -/
-def extract (s : Pos w) (t : IccFrom s) (a : IccTo s) (b : IccFrom t)
-    : (s' : Pos (w.extract a.val b.val)) × IccFrom s' :=
-  ⟨⟨s.val - a.val, ⟨Nat.zero_le (s.val - a.val), by
-    simp only [List.extract_eq_drop_take, List.length_take, List.length_drop,
-      le_inf_iff, tsub_le_iff_right]
-    rw [Nat.sub_add_cancel (le_trans a.is_le (le_trans t.is_ge b.is_ge))]
-    rw [Nat.sub_add_cancel (le_trans a.is_le s.is_le)]
-    exact ⟨le_trans t.is_ge b.is_ge, s.is_le⟩⟩⟩,
-  ⟨t.val - a.val, ⟨by
-    simp only [tsub_le_iff_right]
-    rw [Nat.sub_add_cancel (le_trans a.is_le t.is_ge)]
-    exact t.is_ge,
-  by
-    simp only [List.extract_eq_drop_take, List.length_take, List.length_drop,
-      le_inf_iff, tsub_le_iff_right]
-    rw [Nat.sub_add_cancel (le_trans a.is_le (le_trans t.is_ge b.is_ge))]
-    rw [Nat.sub_add_cancel (le_trans a.is_le s.is_le)]
-    exact ⟨b.is_ge, t.is_le⟩
-    ⟩⟩⟩
-
-omit deq in
-@[simp] theorem extract_fst_val
-    (s : Pos w) (t : IccFrom s) (a : IccTo s) (b : IccFrom t)
-    : (s.extract t a b).fst.val = s.val - a.val := rfl
-
-omit deq in
-@[simp] theorem extract_snd_val
-    (s : Pos w) (t : IccFrom s) (a : IccTo s) (b : IccFrom t)
-    : (s.extract t a b).snd.val = t.val - a.val := rfl
-
-omit deq in
-theorem extract_fst_eq (s : Pos w) (t t' : IccFrom s) (a : IccTo s) (b : IccFrom t)
-    (hb : t'.val ≤ b.val)
-    : (s.extract t a b).fst = (s.extract t' a ⟨b.val, ⟨hb, b.is_le⟩⟩).fst := by rfl
-
---/-- Given a subinterval `s, t`, computes the new subinterval `s', t'`
---in word `wa ++ w ++ wb` that exactly contains `w` -/
---def recycle (s : Pos w) (t : Pos w) (wa wb : List α)
---    : Pos (wa ++ w.extract s.val t.val ++ wb) ×
---      Pos (wa ++ w.extract s.val t.val ++ wb) :=
---  ⟨⟨wa.length, ⟨Nat.zero_le _, by simp⟩⟩,
---  ⟨wa.length + (t.val - s.val), ⟨Nat.zero_le _, by
---    rw [List.length_append, List.length_append, List.length_extract_icc']
---    simp⟩⟩⟩
-
-/-- Given a position `s` in a subinterval `a, b`, computes the new position `s'`
-in word `wa ++ w.extract a b ++ wb` with the corresponding position -/
-def recycle (s a b : Pos w) (hb : s ≤ b) (wa wb : List α)
-    : Pos (wa ++ w.extract a.val b.val ++ wb) :=
-  ⟨wa.length + (s.val - a.val), ⟨Nat.zero_le _, by
-      rw [List.length_append, List.length_append, List.length_extract_icc', add_assoc]
-      refine Nat.add_le_add_left (Nat.le_add_right_of_le ?_) wa.length
-      apply Nat.sub_le_sub_right (val_le_val.mp hb)
-    ⟩⟩
-
-omit deq in
-@[simp] theorem recycle_val {s a b : Pos w} {hb : s ≤ b} {wa wb : List α}
-    : (s.recycle a b hb wa wb).val = wa.length + (s.val - a.val) := rfl
-
---theorem extract_eq {s : Pos w} {t t' : IccFrom s} {a a' : IccTo s}
---    {b : IccFrom t} {b' : IccFrom t'}
---    (ht : t.val = t'.val) (ha : a.val = a'.val) (hb : b.val = b'.val)
---    : s.extract t a b = hb ▸ ha ▸ s.extract t' a' b' := by
---  ext
---  simp [← val_inj, eqRec_eq_cast]
-
-/-- The lower bound -/
-def start (s : Icc a b) : Icc a b := ⟨a, ⟨le_refl a, le_trans s.is_ge s.is_le⟩⟩
-
-/-- The upper bound -/
-def end' (s : Icc a b) : Icc a b := ⟨b, ⟨le_trans s.is_ge s.is_le, le_refl b⟩⟩
-
-@[simp] theorem start_val (s : Icc a b) : s.start.val = a := rfl
-@[simp] theorem end'_val (s : Icc a b) : s.end'.val = b := rfl
-
-@[simp] theorem start_eq {s : Icc a b} (t : Icc a b) : s.start = t.start := rfl
-@[simp] theorem end'_eq {s : Icc a b} (t : Icc a b) : s.end' = t.end' := rfl
-
-theorem start_le (s t : Icc a b) : t.start ≤ s := s.is_ge
-theorem le_end' (s t : Icc a b) : s ≤ t.end' := s.is_le
-
-/-- Distance to the upper bound -/
-def distToEnd (s : Icc a b) := s.end'.val - s.val
-
-theorem distToEnd_lt {s t : Icc a b} : s < t ↔ distToEnd t < distToEnd s := by
-  have leend := t.is_le
-  simp only [distToEnd, val_lt_val, end']
-  omega
-
-theorem distToEnd_le {s t : Icc a b} : s ≤ t ↔ distToEnd t ≤ distToEnd s := by
-  rw [← not_lt, ← not_lt, not_iff_not]
-  exact distToEnd_lt
-
-omit deq
-theorem zero_end' : w = [] ↔ (0 : Pos w) = (0 : Pos w).end' := by
-  rw [← Subtype.val_inj, zero_val, end'_val, (eq_comm : 0 = w.length ↔ _)]
-  exact Iff.symm List.length_eq_zero_iff
-
-def strongRecEnd {motive : Icc a b → Sort u}
-    (ind : ∀ s, (∀ s', s < s' → motive s') → motive s) (s : Icc a b)
-    : motive s :=
-  ind s fun t _lt ↦ strongRecEnd ind t
-termination_by s.distToEnd
-decreasing_by exact distToEnd_lt.mp _lt
-
---def succOfIndex {s : Pos w} {c : α} (hs : w[s.val]? = c) : IccFrom s :=
---  ⟨s.val + 1, ⟨Nat.le_add_right s.val 1, by
+--/-- Probably easier to work with than `Fin` and subtyping at the same time.
+--`Icc a b` is the subtype of natural numbers `n` where `a ≤ n ≤ b`. -/
+--def Icc (a b : ℕ) := {x : ℕ // a ≤ x ∧ x ≤ b}
+--  deriving LE, LT, DecidableEq, Repr, Min, Max, LinearOrder,
+--    Std.LawfulOrderMin, Std.LawfulOrderMax
+--instance Icc.decLt {a b : ℕ} (i j : Icc a b) : Decidable (LT.lt i j) := Nat.decLt ..
+--instance Icc.decLe {a b : ℕ} (i j : Icc a b) : Decidable (LE.le i j) := Nat.decLe ..
+--
+--section Icc
+--
+--variable {a b : ℕ}
+--
+--/-- A valid position in a string `w` (including the end) -/
+--@[reducible] def Pos (w : List α) := Icc 0 w.length deriving Repr
+--/-- A position from `c` to `b` -/
+--@[reducible] def IccFrom (c : Icc a b) := Icc c.val b deriving Repr
+--/-- A position from `a` to `c` -/
+--@[reducible] def IccTo (c : Icc a b) := Icc a c.val deriving Repr
+--
+--namespace Icc
+--
+--theorem val_inj {s t : Icc a b} : s.val = t.val ↔ s = t := Subtype.val_inj
+--theorem val_le_val {s t : Icc a b} : s ≤ t ↔ s.val ≤ t.val := by simp
+--theorem val_lt_val {s t : Icc a b} : s < t ↔ s.val < t.val := by simp
+--
+--theorem is_ge (s : Icc a b) : a ≤ s.val := s.property.left
+--theorem is_le (s : Icc a b) : s.val ≤ b := s.property.right
+--
+--end Icc
+--
+--omit deq in
+--/-- The length of a list extraction using valid positions `s` and `t ≥ s`
+--is just `t - s` with no underflow -/
+--@[simp] theorem _root_.List.length_extract_icc (w : List α) (s : Pos w) (t : IccFrom s)
+--    : (w.extract s.val t.val).length + s.val = t.val := by
+--  simp only [List.extract_eq_drop_take, List.length_take, List.length_drop]
+--  have mints : min (t.val - s.val) (w.length - s.val) = t.val - s.val := by
+--    rw [min_eq_iff]
+--    exact Or.inl ⟨rfl, (Nat.sub_le_sub_iff_right s.is_le).mpr t.is_le⟩
+--  rw [mints, Nat.sub_add_cancel t.is_ge]
+--
+--omit deq in
+--/-- The length of a list extraction using valid positions `s` and `t ≥ s`
+--is just `t - s` with no underflow -/
+--@[simp] theorem _root_.List.length_extract_nat {w : List α} {s t : ℕ}
+--    (hs : s ≤ t) (ht : t ≤ w.length)
+--    : (w.extract s t).length + s = t := by
+--  let spos : Pos w := ⟨s, ⟨Nat.zero_le _, .trans hs ht⟩⟩
+--  let tpos : IccFrom spos := ⟨t, ⟨hs, ht⟩⟩
+--  have lex := List.length_extract_icc w spos tpos
+--  simp only [spos, tpos] at lex
+--  exact lex
+--
+----@[simp] theorem root_.List.min?_append (as bs : List α) (d : α)
+----    : (as ++ bs).min? = as.m
+--
+--omit deq in
+--/-- The length of a list extraction using valid positions `s` and `t`
+--is just `t - s`, potentially with underflow -/
+--@[simp] theorem _root_.List.length_extract_icc' (w : List α) (s : Pos w) (t : Pos w)
+--    : (w.extract s.val t.val).length = t.val - s.val := by
+--  simp only [List.extract_eq_drop_take, List.length_take, List.length_drop,
+--    inf_eq_left, tsub_le_iff_right]
+--  rw [Nat.sub_add_cancel s.prop.2]
+--  exact t.prop.2
+--
+--omit deq in
+--/-- The length of a list extraction using valid positions `s` and `t`
+--is just `t - s`, potentially with underflow -/
+--@[simp] theorem _root_.List.length_extract_nat' {w : List α} {s t : ℕ}
+--    (hs : s ≤ w.length) (ht : t ≤ w.length)
+--    : (w.extract s t).length = t - s :=
+--  List.length_extract_icc' w ⟨s, ⟨Nat.zero_le _, hs⟩⟩ ⟨t, ⟨Nat.zero_le _, ht⟩⟩
+--
+--namespace Icc
+--
+--instance instZero : Zero (Icc 0 b) := ⟨0, ⟨le_refl 0, Nat.zero_le b⟩⟩
+--
+--@[simp] theorem zero_val : (0 : Icc 0 b).val = 0 := rfl
+--
+--/-- Turns `s` into a value bounded by itself and `b` -/
+--def iccFrom (s : Icc a b) : IccFrom s := ⟨s.val, ⟨le_refl s.val, s.is_le⟩⟩
+--
+--/-- Turns `s` into a value bounded by `a` and itself -/
+--def iccTo (s : Icc a b) : IccTo s := ⟨s.val, ⟨s.is_ge, le_refl s.val⟩⟩
+--
+--@[simp] theorem iccFrom_val (s : Icc a b) : s.iccFrom.val = s.val := rfl
+--@[simp] theorem iccTo_val (s : Icc a b) : s.iccTo.val = s.val := rfl
+--
+--theorem le_of_mem_iccFrom {s t : Icc a b} {t' : IccFrom s} (ht : t.val = t'.val)
+--    : s.val ≤ t.val := ht ▸ t'.is_ge
+--
+--theorem ne_of_lt_of_mem_iccFrom {s t : Icc a b} (t' : IccFrom s) (ht : t.val < s.val)
+--    : t.val ≠ t'.val := by
+--  contrapose! ht
+--  exact le_of_mem_iccFrom ht
+--
+--/-- Expands the bounds of `s` -/
+--def expand (s : Icc a b) {a' b' : ℕ} (ha : a' ≤ a) (hb : b ≤ b') : Icc a' b' :=
+--  ⟨s.val, ⟨le_trans ha s.is_ge, le_trans s.is_le hb⟩⟩
+--
+--/-- Expands the lower bound of `s` -/
+--def expandLeft (s : Icc a b) {a' : ℕ} (ha : a' ≤ a) : Icc a' b :=
+--  s.expand ha (le_refl b)
+--
+--/-- Expands the upper bound of `s` -/
+--def expandRight (s : Icc a b) {b' : ℕ} (hb : b ≤ b') : Icc a b' :=
+--  s.expand (le_refl a) hb
+--
+--/-- Expands the lower bound of `s` to 0 -/
+--def expandZero (s : Icc a b) : Icc 0 b := s.expandLeft (Nat.zero_le a)
+--
+--@[simp] theorem expand_val (s : Icc a b) {a' b' : ℕ} (ha : a' ≤ a) (hb : b ≤ b')
+--    : (s.expand ha hb).val = s.val := by rfl
+--
+--@[simp] theorem expandZero_val (s : Icc a b)
+--    : s.expandZero.val = s.val := by rfl
+--
+--@[simp] theorem expand_eq (s : Icc a b) : s.expand (le_refl a) (le_refl b) = s := rfl
+--
+--@[simp] theorem iccFrom_expandLeft (s : Icc a b) {a' : ℕ} (ha : a' ≤ a)
+--    : IccFrom (s.expandLeft ha) = IccFrom s := rfl
+--
+--@[simp] theorem iccTo_expandRight (s : Icc a b) {b' : ℕ} (hb : b ≤ b')
+--    : IccTo (s.expandRight hb) = IccTo s := rfl
+--
+--@[simp] theorem iccFrom_expandZero (s : Icc a b)
+--    : IccFrom s.expandZero = IccFrom s := rfl
+--
+--/-- Use `s` to expand the lower bound of `s'` to the lower bound of `s` -/
+--def widenLeft {s : Icc a b} (s' : IccFrom s) : Icc a b := s'.expandLeft s.is_ge
+--
+--/-- Use `s` to expand the upper bound of `s'` to the upper bound of `s` -/
+--def widenRight {s : Icc a b} (s' : IccTo s) : Icc a b := s'.expandRight s.is_le
+--
+--def widenLeft' {s : Icc a b} (s' : IccFrom s) (a' : IccTo s) : Icc a'.val b :=
+--  s'.expandLeft a'.is_le
+--
+--def widenRight' {s : Icc a b} (s' : IccTo s) (b' : IccFrom s) : Icc a b'.val :=
+--  s'.expandRight b'.is_ge
+--
+--@[simp] theorem widenLeft_val {s : Icc a b} (s' : IccFrom s)
+--    : (s.widenLeft s').val = s'.val := rfl
+--
+--@[simp] theorem widenRight_val {s : Icc a b} (s' : IccTo s)
+--    : (s.widenRight s').val = s'.val := rfl
+--
+--@[simp] theorem widenLeft'_val {s : Icc a b} (s' : IccFrom s) (a' : IccTo s)
+--    : (s.widenLeft' s' a').val = s'.val := rfl
+--
+--@[simp] theorem widenRight'_val {s : Icc a b} (s' : IccTo s) (b' : IccFrom s)
+--    : (s.widenRight' s' b').val = s'.val := rfl
+--
+--/-- Given a subinterval to restrict positions `s` and `t` to, gives an new `s'` and `t'`
+--for that subinterval -/
+--def extract (s : Pos w) (t : IccFrom s) (a : IccTo s) (b : IccFrom t)
+--    : (s' : Pos (w.extract a.val b.val)) × IccFrom s' :=
+--  ⟨⟨s.val - a.val, ⟨Nat.zero_le (s.val - a.val), by
+--    simp only [List.extract_eq_drop_take, List.length_take, List.length_drop,
+--      le_inf_iff, tsub_le_iff_right]
+--    rw [Nat.sub_add_cancel (le_trans a.is_le (le_trans t.is_ge b.is_ge))]
+--    rw [Nat.sub_add_cancel (le_trans a.is_le s.is_le)]
+--    exact ⟨le_trans t.is_ge b.is_ge, s.is_le⟩⟩⟩,
+--  ⟨t.val - a.val, ⟨by
+--    simp only [tsub_le_iff_right]
+--    rw [Nat.sub_add_cancel (le_trans a.is_le t.is_ge)]
+--    exact t.is_ge,
+--  by
+--    simp only [List.extract_eq_drop_take, List.length_take, List.length_drop,
+--      le_inf_iff, tsub_le_iff_right]
+--    rw [Nat.sub_add_cancel (le_trans a.is_le (le_trans t.is_ge b.is_ge))]
+--    rw [Nat.sub_add_cancel (le_trans a.is_le s.is_le)]
+--    exact ⟨b.is_ge, t.is_le⟩
+--    ⟩⟩⟩
+--
+--omit deq in
+--@[simp] theorem extract_fst_val
+--    (s : Pos w) (t : IccFrom s) (a : IccTo s) (b : IccFrom t)
+--    : (s.extract t a b).fst.val = s.val - a.val := rfl
+--
+--omit deq in
+--@[simp] theorem extract_snd_val
+--    (s : Pos w) (t : IccFrom s) (a : IccTo s) (b : IccFrom t)
+--    : (s.extract t a b).snd.val = t.val - a.val := rfl
+--
+--omit deq in
+--theorem extract_fst_eq (s : Pos w) (t t' : IccFrom s) (a : IccTo s) (b : IccFrom t)
+--    (hb : t'.val ≤ b.val)
+--    : (s.extract t a b).fst = (s.extract t' a ⟨b.val, ⟨hb, b.is_le⟩⟩).fst := by rfl
+--
+----/-- Given a subinterval `s, t`, computes the new subinterval `s', t'`
+----in word `wa ++ w ++ wb` that exactly contains `w` -/
+----def recycle (s : Pos w) (t : Pos w) (wa wb : List α)
+----    : Pos (wa ++ w.extract s.val t.val ++ wb) ×
+----      Pos (wa ++ w.extract s.val t.val ++ wb) :=
+----  ⟨⟨wa.length, ⟨Nat.zero_le _, by simp⟩⟩,
+----  ⟨wa.length + (t.val - s.val), ⟨Nat.zero_le _, by
+----    rw [List.length_append, List.length_append, List.length_extract_icc']
+----    simp⟩⟩⟩
+--
+--/-- Given a position `s` in a subinterval `a, b`, computes the new position `s'`
+--in word `wa ++ w.extract a b ++ wb` with the corresponding position -/
+--def recycle (s a b : Pos w) (hb : s ≤ b) (wa wb : List α)
+--    : Pos (wa ++ w.extract a.val b.val ++ wb) :=
+--  ⟨wa.length + (s.val - a.val), ⟨Nat.zero_le _, by
+--      rw [List.length_append, List.length_append, List.length_extract_icc', add_assoc]
+--      refine Nat.add_le_add_left (Nat.le_add_right_of_le ?_) wa.length
+--      apply Nat.sub_le_sub_right (val_le_val.mp hb)
+--    ⟩⟩
+--
+--omit deq in
+--@[simp] theorem recycle_val {s a b : Pos w} {hb : s ≤ b} {wa wb : List α}
+--    : (s.recycle a b hb wa wb).val = wa.length + (s.val - a.val) := rfl
+--
+----theorem extract_eq {s : Pos w} {t t' : IccFrom s} {a a' : IccTo s}
+----    {b : IccFrom t} {b' : IccFrom t'}
+----    (ht : t.val = t'.val) (ha : a.val = a'.val) (hb : b.val = b'.val)
+----    : s.extract t a b = hb ▸ ha ▸ s.extract t' a' b' := by
+----  ext
+----  simp [← val_inj, eqRec_eq_cast]
+--
+--/-- The lower bound -/
+--def start (s : Icc a b) : Icc a b := ⟨a, ⟨le_refl a, le_trans s.is_ge s.is_le⟩⟩
+--
+--/-- The upper bound -/
+--def end' (s : Icc a b) : Icc a b := ⟨b, ⟨le_trans s.is_ge s.is_le, le_refl b⟩⟩
+--
+--@[simp] theorem start_val (s : Icc a b) : s.start.val = a := rfl
+--@[simp] theorem end'_val (s : Icc a b) : s.end'.val = b := rfl
+--
+--@[simp] theorem start_eq {s : Icc a b} (t : Icc a b) : s.start = t.start := rfl
+--@[simp] theorem end'_eq {s : Icc a b} (t : Icc a b) : s.end' = t.end' := rfl
+--
+--theorem start_le (s t : Icc a b) : t.start ≤ s := s.is_ge
+--theorem le_end' (s t : Icc a b) : s ≤ t.end' := s.is_le
+--
+--/-- Distance to the upper bound -/
+--def distToEnd (s : Icc a b) := s.end'.val - s.val
+--
+--theorem distToEnd_lt {s t : Icc a b} : s < t ↔ distToEnd t < distToEnd s := by
+--  have leend := t.is_le
+--  simp only [distToEnd, val_lt_val, end']
+--  omega
+--
+--theorem distToEnd_le {s t : Icc a b} : s ≤ t ↔ distToEnd t ≤ distToEnd s := by
+--  rw [← not_lt, ← not_lt, not_iff_not]
+--  exact distToEnd_lt
+--
+--omit deq
+--theorem zero_end' : w = [] ↔ (0 : Pos w) = (0 : Pos w).end' := by
+--  rw [← Subtype.val_inj, zero_val, end'_val, (eq_comm : 0 = w.length ↔ _)]
+--  exact Iff.symm List.length_eq_zero_iff
+--
+--def strongRecEnd {motive : Icc a b → Sort u}
+--    (ind : ∀ s, (∀ s', s < s' → motive s') → motive s) (s : Icc a b)
+--    : motive s :=
+--  ind s fun t _lt ↦ strongRecEnd ind t
+--termination_by s.distToEnd
+--decreasing_by exact distToEnd_lt.mp _lt
+--
+----def succOfIndex {s : Pos w} {c : α} (hs : w[s.val]? = c) : IccFrom s :=
+----  ⟨s.val + 1, ⟨Nat.le_add_right s.val 1, by
+----    rw [List.getElem?_eq_some_iff] at hs
+----    rcases hs with ⟨hs, _⟩
+----    exact Nat.add_one_le_of_lt hs
+----  ⟩⟩
+--
+--/-- Use the fact that an item exists at `w[s]` to provably add 1 to `s` -/
+--def succOfIndex {s : Pos w} {c : α} (hs : w[s.val]? = c) : Pos w :=
+--  ⟨s.val + 1, ⟨Nat.zero_le _, by
 --    rw [List.getElem?_eq_some_iff] at hs
 --    rcases hs with ⟨hs, _⟩
 --    exact Nat.add_one_le_of_lt hs
 --  ⟩⟩
-
-/-- Use the fact that an item exists at `w[s]` to provably add 1 to `s` -/
-def succOfIndex {s : Pos w} {c : α} (hs : w[s.val]? = c) : Pos w :=
-  ⟨s.val + 1, ⟨Nat.zero_le _, by
-    rw [List.getElem?_eq_some_iff] at hs
-    rcases hs with ⟨hs, _⟩
-    exact Nat.add_one_le_of_lt hs
-  ⟩⟩
-
-omit deq in
-@[simp] theorem succOfIndex_val {s : Pos w} {c : α} (hs : w[s.val]? = c)
-    : (succOfIndex hs).val = s.val + 1 := by rfl
-
+--
+--omit deq in
+--@[simp] theorem succOfIndex_val {s : Pos w} {c : α} (hs : w[s.val]? = c)
+--    : (succOfIndex hs).val = s.val + 1 := by rfl
+--
+----def addOfIndex {s : Pos w} {t : ℕ} {cs : List α}
+----    (ex : w.extract s.val (s.val + t) = cs) (hcs : cs.length = t) : IccFrom s :=
+----  ⟨s.val + t, ⟨Nat.le_add_right s.val t, by
+----    rw [← ex, List.extract_eq_drop_take, Nat.add_sub_cancel_left] at hcs
+----    have tle := hcs ▸ List.length_take_le' t (List.drop s.val w)
+----    rw [List.length_drop] at tle
+----    exact Nat.add_le_of_le_sub' s.is_le tle
+----  ⟩⟩
+--
+--/-- Use the fact that the subsequence at position `s` with length `t`
+--actually has length `t` to provably add `t` to `s` -/
 --def addOfIndex {s : Pos w} {t : ℕ} {cs : List α}
---    (ex : w.extract s.val (s.val + t) = cs) (hcs : cs.length = t) : IccFrom s :=
---  ⟨s.val + t, ⟨Nat.le_add_right s.val t, by
+--    (ex : w.extract s.val (s.val + t) = cs) (hcs : cs.length = t) : Pos w :=
+--  ⟨s.val + t, ⟨Nat.zero_le _, by
 --    rw [← ex, List.extract_eq_drop_take, Nat.add_sub_cancel_left] at hcs
 --    have tle := hcs ▸ List.length_take_le' t (List.drop s.val w)
 --    rw [List.length_drop] at tle
 --    exact Nat.add_le_of_le_sub' s.is_le tle
 --  ⟩⟩
-
-/-- Use the fact that the subsequence at position `s` with length `t`
-actually has length `t` to provably add `t` to `s` -/
-def addOfIndex {s : Pos w} {t : ℕ} {cs : List α}
-    (ex : w.extract s.val (s.val + t) = cs) (hcs : cs.length = t) : Pos w :=
-  ⟨s.val + t, ⟨Nat.zero_le _, by
-    rw [← ex, List.extract_eq_drop_take, Nat.add_sub_cancel_left] at hcs
-    have tle := hcs ▸ List.length_take_le' t (List.drop s.val w)
-    rw [List.length_drop] at tle
-    exact Nat.add_le_of_le_sub' s.is_le tle
-  ⟩⟩
-
-omit deq in
-@[simp] theorem addOfIndex_val {s : Pos w} {t : ℕ} {cs : List α}
-    {ex : w.extract s.val (s.val + t) = cs} {hcs : cs.length = t}
-    : (addOfIndex ex hcs).val = s.val + t := by rfl
-
-end Icc
-
---theorem List.getElem?_extract_lt (w : List α) (s : Pos w) (t : IccFrom s)
-
-end Icc
-
-omit deq in
-/-- Pasting two extracts together where the second one starts where the
-first one ends -/
-@[simp] theorem _root_.List.extract_append_extract' {s t u : ℕ}
-    (hs : s ≤ t) (ht : t ≤ u) (hu : u ≤ w.length)
-    : w.extract s t ++ w.extract t u = w.extract s u := by
-  simp only [List.extract_eq_drop_take]
-  rw (occs := [1, 3]) [← List.take_append_drop u w]
-  rw [List.drop_append]
-  rw [List.take_append_of_le_length ?st, List.take_append_of_le_length ?su];
-  case st | su =>
-    simp only [List.length_drop, List.length_take, tsub_le_iff_right, min_eq_left_iff.mpr hu]
-    rw [Nat.sub_add_cancel] <;> first | exact le_refl _ | assumption | exact .trans hs ht
-  rw [List.take_drop (i := u - t), List.drop_take, ← List.extract_eq_drop_take,
-    Nat.add_sub_cancel' ht]
-  rw (occs := [2]) [← List.take_append_drop s w]
-  rw [List.take_append, List.take_take (i := u), min_eq_right_iff.mpr (.trans hs ht),
-    List.length_take, min_eq_left_iff.mpr (.trans hs <| .trans ht hu),
-    List.drop_append, List.drop_eq_nil_iff.mpr]; rotate_right
-  · simp only [List.length_take, inf_le_iff]; exact Or.inl hs
-  simp only [List.extract_eq_drop_take, List.length_take, List.nil_append,
-    min_eq_left_iff.mpr (.trans hs <| .trans ht hu)]
-  rw [← List.extract_eq_drop_take, List.take_append_drop]
-  simp
-
-omit deq in
-@[simp] theorem _root_.List.extract_append_extract {s t u : Pos w}
-    (hs : s ≤ t) (ht : t ≤ u) :
-    w.extract s.val t.val ++ w.extract t.val u.val = w.extract s.val u.val :=
-  List.extract_append_extract' (Icc.val_le_val.mp hs) (Icc.val_le_val.mp ht) u.is_le
-
-omit deq in
-theorem _root_.List.extract_append_extract_assoc_right {s t u : Pos w}
-    (hs : s ≤ t) (ht : t ≤ u) (wa wb)
-    : wa ++ w.extract s.val t.val ++ (w.extract t.val u.val ++ wb) =
-      wa ++ w.extract s.val u.val ++ wb := by
-  rw [← List.append_assoc, List.append_assoc wa, List.extract_append_extract hs ht]
-
-omit deq in
-theorem _root_.List.extract_append_extract_assoc_left {s t u : Pos w}
-    (hs : s ≤ t) (ht : t ≤ u) (wa wb)
-    : (wa ++ w.extract s.val t.val) ++ w.extract t.val u.val ++ wb =
-      wa ++ w.extract s.val u.val ++ wb := by
-  rw [List.append_assoc wa, List.extract_append_extract hs ht]
-
-namespace Icc
-
-omit deq in
-theorem recycle_extract_append_right {s t a b : Pos w} (as : a ≤ s) (st : s ≤ t)
-    (tb : t ≤ b) (wa wb : List α)
-    : s.recycle a t st wa (w.extract t.val b.val ++ wb) =
-    List.extract_append_extract_assoc_right (.trans as st) tb wa wb ▸
-      s.recycle a b (.trans st tb) wa wb := by
-  rw [eqRec_eq_cast, eq_comm, cast_eq_iff_heq, Subtype.heq_iff_coe_eq]
-  · simp
-  simp [List.extract_append_extract_assoc_right (.trans as st) tb]
-
-omit deq in
-theorem recycle_extract_append_left {s t a b : Pos w} (at' : a ≤ t) (ts : t ≤ s)
-    (sb : s ≤ b) (wa wb : List α)
-    : s.recycle t b sb (wa ++ w.extract a.val t.val) wb =
-    List.extract_append_extract_assoc_left at' (.trans ts sb) wa wb ▸
-      s.recycle a b sb wa wb := by
-  rw [eqRec_eq_cast, eq_comm, cast_eq_iff_heq, Subtype.heq_iff_coe_eq]
-  · simp only [List.extract_eq_drop_take, recycle_val, List.length_append, List.length_take,
-      List.length_drop]
-    rw [add_assoc, Nat.add_right_inj, min_eq_left_iff.mpr (Nat.sub_le_sub_right t.is_le _)]
-    rw [add_comm, Nat.sub_add_sub_cancel ts at']
-  rw [List.extract_append_extract_assoc_left at' (.trans ts sb)]
-  simp
+--
+--omit deq in
+--@[simp] theorem addOfIndex_val {s : Pos w} {t : ℕ} {cs : List α}
+--    {ex : w.extract s.val (s.val + t) = cs} {hcs : cs.length = t}
+--    : (addOfIndex ex hcs).val = s.val + t := by rfl
+--
+--end Icc
+--
+----theorem List.getElem?_extract_lt (w : List α) (s : Pos w) (t : IccFrom s)
+--
+--end Icc
+--
+--omit deq in
+--/-- Pasting two extracts together where the second one starts where the
+--first one ends -/
+--@[simp] theorem _root_.List.extract_append_extract' {s t u : ℕ}
+--    (hs : s ≤ t) (ht : t ≤ u) (hu : u ≤ w.length)
+--    : w.extract s t ++ w.extract t u = w.extract s u := by
+--  simp only [List.extract_eq_drop_take]
+--  rw (occs := [1, 3]) [← List.take_append_drop u w]
+--  rw [List.drop_append]
+--  rw [List.take_append_of_le_length ?st, List.take_append_of_le_length ?su];
+--  case st | su =>
+--    simp only [List.length_drop, List.length_take, tsub_le_iff_right, min_eq_left_iff.mpr hu]
+--    rw [Nat.sub_add_cancel] <;> first | exact le_refl _ | assumption | exact .trans hs ht
+--  rw [List.take_drop (i := u - t), List.drop_take, ← List.extract_eq_drop_take,
+--    Nat.add_sub_cancel' ht]
+--  rw (occs := [2]) [← List.take_append_drop s w]
+--  rw [List.take_append, List.take_take (i := u), min_eq_right_iff.mpr (.trans hs ht),
+--    List.length_take, min_eq_left_iff.mpr (.trans hs <| .trans ht hu),
+--    List.drop_append, List.drop_eq_nil_iff.mpr]; rotate_right
+--  · simp only [List.length_take, inf_le_iff]; exact Or.inl hs
+--  simp only [List.extract_eq_drop_take, List.length_take, List.nil_append,
+--    min_eq_left_iff.mpr (.trans hs <| .trans ht hu)]
+--  rw [← List.extract_eq_drop_take, List.take_append_drop]
+--  simp
+--
+--omit deq in
+--@[simp] theorem _root_.List.extract_append_extract {s t u : Pos w}
+--    (hs : s ≤ t) (ht : t ≤ u) :
+--    w.extract s.val t.val ++ w.extract t.val u.val = w.extract s.val u.val :=
+--  List.extract_append_extract' (Icc.val_le_val.mp hs) (Icc.val_le_val.mp ht) u.is_le
+--
+--omit deq in
+--theorem _root_.List.extract_append_extract_assoc_right {s t u : Pos w}
+--    (hs : s ≤ t) (ht : t ≤ u) (wa wb)
+--    : wa ++ w.extract s.val t.val ++ (w.extract t.val u.val ++ wb) =
+--      wa ++ w.extract s.val u.val ++ wb := by
+--  rw [← List.append_assoc, List.append_assoc wa, List.extract_append_extract hs ht]
+--
+--omit deq in
+--theorem _root_.List.extract_append_extract_assoc_left {s t u : Pos w}
+--    (hs : s ≤ t) (ht : t ≤ u) (wa wb)
+--    : (wa ++ w.extract s.val t.val) ++ w.extract t.val u.val ++ wb =
+--      wa ++ w.extract s.val u.val ++ wb := by
+--  rw [List.append_assoc wa, List.extract_append_extract hs ht]
+--
+--namespace Icc
+--
+--omit deq in
+--theorem recycle_extract_append_right {s t a b : Pos w} (as : a ≤ s) (st : s ≤ t)
+--    (tb : t ≤ b) (wa wb : List α)
+--    : s.recycle a t st wa (w.extract t.val b.val ++ wb) =
+--    List.extract_append_extract_assoc_right (.trans as st) tb wa wb ▸
+--      s.recycle a b (.trans st tb) wa wb := by
+--  rw [eqRec_eq_cast, eq_comm, cast_eq_iff_heq, Subtype.heq_iff_coe_eq]
+--  · simp
+--  simp [List.extract_append_extract_assoc_right (.trans as st) tb]
+--
+--omit deq in
+--theorem recycle_extract_append_left {s t a b : Pos w} (at' : a ≤ t) (ts : t ≤ s)
+--    (sb : s ≤ b) (wa wb : List α)
+--    : s.recycle t b sb (wa ++ w.extract a.val t.val) wb =
+--    List.extract_append_extract_assoc_left at' (.trans ts sb) wa wb ▸
+--      s.recycle a b sb wa wb := by
+--  rw [eqRec_eq_cast, eq_comm, cast_eq_iff_heq, Subtype.heq_iff_coe_eq]
+--  · simp only [List.extract_eq_drop_take, recycle_val, List.length_append, List.length_take,
+--      List.length_drop]
+--    rw [add_assoc, Nat.add_right_inj, min_eq_left_iff.mpr (Nat.sub_le_sub_right t.is_le _)]
+--    rw [add_comm, Nat.sub_add_sub_cancel ts at']
+--  rw [List.extract_append_extract_assoc_left at' (.trans ts sb)]
+--  simp
 
 --omit deq in
 --theorem recycle_extract_append' {s t a b : Pos w} (as : a ≤ s) (st : s ≤ t)
@@ -418,8 +420,8 @@ theorem recycle_extract_append_left {s t a b : Pos w} (at' : a ≤ t) (ts : t �
 --  rw [eqRec_eq_cast, eq_comm, cast_eq_iff_heq, Subtype.heq_iff_coe_eq]
 --  · simp
 --  simp [List.extract_append_extract_assoc hs ht]
-
-end Icc
+--
+--end Icc
 
 --def Pos (w : List α) := Icc 0 w.length
 --  deriving LE, LT, DecidableEq, DecidableLE, DecidableLT, Repr
@@ -551,28 +553,28 @@ end Icc
 /-- A *capture* is a stack of substring positions.
 Most programming languages treat this as an `option`,
 having only 0 or 1 items on it, but .NET is different. -/
-def Capture (w : List α) := List (Pos w × Pos w) deriving DecidableEq, Repr
+def Capture := List (ℕ × ℕ) deriving DecidableEq, Repr
 
-instance Capture.instZero : Zero (Capture w) where
+instance Capture.instZero : Zero Capture where
   zero := []
 
 /-- A map from "names" (actually natural numbers) to captures -/
-def Captures (w : List α) := ℕ →₀ Capture w deriving Zero, DFunLike
+def Captures := ℕ →₀ Capture deriving Zero, DFunLike
 
 namespace Captures
 
 omit deq in
-@[simp] theorem zero_get {w : List α} {n : ℕ} : (0 : Captures w) n = [] := by rfl
+@[simp] theorem zero_get {n : ℕ} : (0 : Captures) n = [] := by rfl
 
 /-- Turns this into a list of (index, capture) pairs -/
-def toList (cs : Captures w) : List (ℕ × Capture w) :=
+def toList (cs : Captures) : List (ℕ × Capture) :=
   (fun n => (n, cs n)) <$> cs.support.sort
 
-instance instRepr : Repr (Captures w) where
+instance instRepr : Repr Captures where
   reprPrec cs := cs.toList.repr
 
 /-- Because `Finsupp.update` is noncomputable even in cases it doesn't need to be -/
-def update (cs : Captures w) (n : ℕ) (c : Capture w) : Captures w :=
+def update (cs : Captures) (n : ℕ) (c : Capture) : Captures :=
   Finsupp.mk
     (support := if c = 0 then cs.support \ {n} else cs.support ∪ {n})
     (toFun := Function.update cs.toFun n c)
@@ -589,16 +591,16 @@ def update (cs : Captures w) (n : ℕ) (c : Capture w) : Captures w :=
 
 end Captures
 
-omit deq in
-theorem length_extract_pos_posFrom (s : Pos w) (s' : IccFrom s)
-    : (w.extract s.val s'.val).length = s'.val - s.val := by
-  rw [List.extract_eq_drop_take]
-  apply List.length_take_of_le
-  rw [List.length_drop]
-  apply Nat.sub_le_sub_right s'.is_le
+--omit deq in
+--theorem length_extract_pos_posFrom (s : Pos w) (s' : IccFrom s)
+--    : (w.extract s.val s'.val).length = s'.val - s.val := by
+--  rw [List.extract_eq_drop_take]
+--  apply List.length_take_of_le
+--  rw [List.length_drop]
+--  apply Nat.sub_le_sub_right s'.is_le
 
 /-- A list of partial matches ((pos × captures) pairs) -/
-@[reducible] def PartialMatches (w : List α) := List (Pos w × Captures w)
+@[reducible] def PartialMatches := List (ℕ × Captures)
   deriving Repr
 
 end Regex
