Regex/Lemmas/Bounds.lean
@@ -1,0 +1,145 @@
+import Regex.Basic
+
+/-! Lemmas about the bounds of matches. We also prove a convenient conditional
+version of `star_terminates` -/
+
+namespace Regex
+
+variable {α : Type u} [deq : DecidableEq α] {r : Regex α} {w : List α}
+  {s : ℕ} {cap : Captures} {term : r.Terminates w s cap}
+
+def decreasingStrongRec {n : ℕ} {motive : (m : ℕ) → m ≤ n → Sort u}
+    (ind : ∀ m, (mn : m ≤ n) →
+      (∀ k, (kn : k ≤ n) → (km : k > m) → motive k kn) →
+      motive m mn)
+    (m : ℕ) (mn : m ≤ n)
+    : motive m mn :=
+  ind m mn fun k kn _ ↦ decreasingStrongRec ind k kn
+
+/-- The property that all matches that end in bounds. -/
+def EndsInBounds (r : Regex α) (w : List α) (s : ℕ) (cap : Captures)
+    (term : r.Terminates w s cap) :=
+    ∀ {mat},
+      mat ∈ r.matchPartial w s cap term → mat.1 ≤ w.length
+
+--/-- If a start index that is at most `w.length` is supplied (i.e. is in bounds),
+--then all matches end in bounds. -/
+--theorem matchPartial_inBounds_le (hs : s ≤ w.length) : r.EndsInBounds w s cap term := by
+--  revert term
+--  induction s, hs using decreasingStrongRec generalizing cap with | ind s slt ind =>
+--    intro term
+--    induction r with
+--    | bot => simp [matchPartial_bot] at mem
+--    | empty => simp [matchPartial_empty, Prod.eq_iff_fst_eq_snd_eq] at ind mem; simp [mem, slt]
+--    | unit _ =>
+--      simp only [matchPartial_unit, List.getElem?_eq_some_iff, List.mem_ite_nil_right, List.mem_cons,
+--        List.not_mem_nil, or_false] at mem
+--      rcases mem with ⟨⟨lt, _⟩, mateq⟩
+--      simp [mateq, lt]
+--    | concat q r qind rind =>
+--      simp [matchPartial_concat] at ind mem
+--      rcases mem with ⟨s', cap', qmem, rmem⟩
+--      specialize qind hs qmem
+--      simp only at qind
+--      exact rind qind rmem
+--    | or q r qind rind =>
+--      simp only [matchPartial_or, List.mem_append] at mem
+--      exact Or.casesOn mem (fun mem ↦ qind hs mem) (fun mem ↦ rind hs mem)
+--    | filterEmpty _ r rind =>
+--      simp only [matchPartial_filterEmpty, ge_iff_le, eq_iff_iff, Bool.decide_iff_dist,
+--        Bool.decide_eq_true, List.mem_filter, beq_iff_eq] at mem
+--      exact rind hs mem.1
+--    | star t r rind =>
+--      simp only [matchPartial_star] at mem
+--      cases t
+--      case greedy | lazy =>
+--        simp [matchPartial_or, matchPartial_concat, matchPartial_filterEmpty,
+--          matchPartial_empty] at mem
+--        try rw [or_comm (a := mat = _), or_assoc] at mem
+--        rcases mem with mem | ⟨s', cap', mem', _⟩ | eq
+--        · exact rind hs mem.1
+--        · specialize rind hs mem'.1; simp only at rind; exact _
+--        · simp [eq]
+
+/-- If a start index that is `w.length` or out of bounds is supplied,
+there are no positive-length matches. -/
+theorem matchPartial_outOfBounds_eq {term : r.Terminates w s cap}
+    (hs : w.length ≤ s) {mat} (mem : mat ∈ r.matchPartial w s cap term)
+    : s = mat.1 := by
+  induction r generalizing s cap mat with
+  | bot => simp [matchPartial_bot] at mem
+  | empty => simp [matchPartial_empty] at mem; simp [mem]
+  | unit _ =>
+    simp only [matchPartial_unit, List.mem_ite_nil_right, List.mem_cons, List.not_mem_nil,
+      or_false] at mem
+    rw [List.getElem?_eq_some_iff] at mem
+    rcases mem with ⟨⟨lt, _⟩, _⟩
+    exact (not_lt.mpr hs lt).elim
+  | concat q r qind rind =>
+    simp only [matchPartial_concat, List.mem_flatten, List.mem_pmap, Prod.exists, ↓existsAndEq,
+      true_and] at mem
+    rcases mem with ⟨s', cap', qmem, rmem⟩
+    specialize qind hs qmem
+    simp only at qind
+    specialize rind (qind ▸ hs) rmem
+    rw [← rind, ← qind]
+  | or q r qind rind =>
+    simp only [matchPartial_or, List.mem_append] at mem
+    exact Or.casesOn mem (fun mem ↦ qind hs mem) (fun mem ↦ rind hs mem)
+  | filterEmpty _ r rind =>
+    simp only [matchPartial_filterEmpty, ge_iff_le, eq_iff_iff, Bool.decide_iff_dist,
+      Bool.decide_eq_true, List.mem_filter, beq_iff_eq] at mem
+    exact rind hs mem.1
+  | star t r rind =>
+    simp only [matchPartial_star] at mem
+    cases t
+    case greedy | lazy =>
+      simp only [matchPartial_or, matchPartial_filterEmpty, ge_iff_le, eq_iff_iff, iff_true,
+        matchPartial_concat, Bool.false_eq_true, iff_false, not_le, matchPartial_empty,
+        List.append_assoc, List.mem_append, List.mem_filter, decide_eq_true_eq, List.mem_flatten,
+        List.mem_pmap, Prod.exists, ↓existsAndEq, true_and, List.mem_cons, List.not_mem_nil,
+        or_false] at mem
+      try rw [or_comm (a := mat = _), or_assoc] at mem
+      rcases mem with mem | ⟨s', cap', mem', _⟩ | eq
+      · exact rind hs mem.1
+      · specialize rind hs mem'.1; simp only at rind; exact
+          (not_lt_iff_eq_or_lt.mpr (Or.inl rind) mem'.2).elim
+      · simp [eq]
+  | start => simp [matchPartial_start] at mem; simp [mem]
+  | end' => simp [matchPartial_end'] at mem; simp [mem]
+  | capture _ r rind =>
+    simp only [matchPartial_capture, List.mem_map, Prod.exists] at mem
+    rcases mem with ⟨s', cap', mem, up⟩
+    specialize rind hs mem
+    rw [Prod.eq_iff_fst_eq_snd_eq] at up
+    simp at up
+    simp [up, rind]
+  | backref d _ =>
+    simp only [matchPartial_backref, List.extract_eq_drop_take, List.length_take, List.length_drop,
+      add_tsub_cancel_left] at mem
+    split at mem
+    · split at mem <;> (simp at mem; try simp [mem])
+    · split at mem <;> (expose_names; simp only [List.mem_cons, List.not_mem_nil, or_false] at mem)
+      simp only [mem, Nat.left_eq_add, Nat.min_eq_zero_iff]
+      simp only [List.drop_eq_nil_iff.mpr hs, List.take_nil, List.nil_eq, List.take_eq_nil_iff,
+        List.drop_eq_nil_iff] at h
+      rwa [← Nat.sub_eq_zero_iff_le] at h
+
+/-- `star t r` terminates if (but not only if)
+`r` terminates for every capture and for every position starting from here -/
+theorem star_terminates_of_forall {t : StarType}
+    : (∀ s' ≥ s, ∀ cap', r.Terminates w s' cap') →
+      [/⟨r⟩*‹t›/].Terminates w s cap := by
+  intro term
+  induction h : w.length - s using Nat.strongRec generalizing s cap with
+  | ind n ind =>
+    rw [star_terminates]
+    refine ⟨term s (le_refl _) cap, fun mat mem lt ↦ ?_⟩
+    simp only [← h] at ind
+    by_cases! h : s < w.length
+    · exact ind (w.length - mat.1) (Nat.sub_lt_sub_left h lt)
+        (fun s' ge ↦ term s' (le_of_lt (Trans.trans lt ge))) rfl
+    · have eq := matchPartial_outOfBounds_eq h mem
+      exact (ne_of_lt lt eq).elim
+
+end Regex
